Finish Ex01a

Ex01a.fst
@@ -1,12 +1,52 @@
 module Ex01a
 
+
+open FStar.Exn
+open FStar.All
+
 type filename = string
 
 let canWrite (f : filename) =
   match f with
-    | "demo/tempfile" -> true
-    | _ -> false
+  | "demo/tempfile" -> true
+  | _ -> false
 
 let canRead (f : filename) =
   canWrite f
   || f = "demo/README"
+
+
+val read : f : filename {canRead f} -> ML string
+let read f = FStar.IO.print_string("Dummy read of file " ^ f ^ "\n"); f
+
+val write : f:filename{canWrite f} -> string -> ML unit
+let write f s = FStar.IO.print_string ("Dummy write of string " ^ s ^ " to file " ^ f ^ "\n")
+
+
+  // BEGIN: UntrustedClientCode
+  let passwd : filename = "demo/password"
+  let readme : filename = "demo/README"
+  let tmp    : filename = "demo/tempfile"
+  // END: UntrustedClientCode
+
+  // BEGIN: StaticChecking
+  val staticChecking : unit -> ML unit
+  let staticChecking () =
+    let v1 = read tmp in
+    let v2 = read readme in
+    // let v3 = read passwd in // invalid read, fails type-checking
+    write tmp "hello!"
+    // ; write passwd "junk" // invalid write , fails type-checking
+  // END: StaticChecking
+
+
+  exception InvalidRead
+  val checkedRead : filename -> ML string
+  let checkedRead f =
+    if canRead f then read f else raise InvalidRead
+
+
+  exception InvalidWrite
+  val checkedWrite : filename -> string -> ML unit
+  let checkedWrite f s =
+    if canWrite f then write f s else raise InvalidWrite
